Refactoring

theories/channel/channel.v
@@ -21,85 +21,88 @@ In this file we define the three message-passing connectives:
 
 It is additionaly shown that the channel ownership [c ↣ prot] is closed under
 the subprotocol relation [⊑] *)
-From iris.algebra Require Import gmap excl_auth gmap_view.
 From iris.heap_lang Require Export primitive_laws notation.
 From iris.heap_lang Require Export proofmode.
 From iris.heap_lang.lib Require Import spin_lock.
-From actris.utils Require Export llist.
-From actris.channel Require Import proto_model.
 From actris.channel Require Export proto.
+From actris.utils Require Import llist skip.
 Set Default Proof Using "Type".
+
+Local Existing Instance spin_lock.
 
 (** * The definition of the message-passing connectives *)
 Definition new_chan : val :=
-  λ: <>, let: "l1" := ref NONEV in
-         let: "l2" := ref NONEV in
-         (("l1","l2"), ("l2","l1")).
+  λ: <>,
+     let: "l" := lnil #() in
+     let: "r" := lnil #() in
+     let: "lk" := newlock #() in
+     ((("l","r"),"lk"), (("r","l"),"lk")).
 
 Definition fork_chan : val := λ: "f",
   let: "cc" := new_chan #() in
   Fork ("f" (Snd "cc"));; Fst "cc".
 
-Definition wait : val :=
-  rec: "go" "l" :=
-    match: !"l" with
-      NONE => #()
-    | SOME <> => "go" "l"
-    end.
-
 Definition send : val :=
   λ: "c" "v",
-    let: "l" := Fst "c" in
-    "l" <- SOME "v";; wait "l".
+    let: "lk" := Snd "c" in
+    let: "l" := Fst (Fst "c") in
+    let: "r" := Snd (Fst "c") in
+    acquire "lk";;
+    lsnoc "l" "v";;
+    release "lk".
 
-(* Definition recv : val := *)
-(*   rec: "go" "c" "i" := *)
-(*     let: "l" := Snd (llookup "c" "i") in *)
-(*     match: !"l" with *)
-(*       NONE => "go" "c" *)
-(*     | SOME "v" => "c" <- NONE;; "v"  *)
-(*     end. *)
+Definition try_recv : val :=
+  λ: "c",
+    let: "lk" := Snd "c" in
+    acquire "lk";;
+    let: "l" := Snd (Fst "c") in
+    let: "ret" := if: lisnil "l" then NONE else SOME (lpop "l") in
+    release "lk";; "ret".
 
 Definition recv : val :=
   rec: "go" "c" :=
-    let: "l" := Snd "c" in
-    let: "v" := Xchg "l" NONEV in
-    match: "v" with
-      NONE => "go" "c"
-    | SOME "v" => "v" 
+    match: try_recv "c" with
+      SOME "p" => "p"
+    | NONE => "go" "c"
     end.
 
+(** * Setup of Iris's cameras *)
 Class chanG Σ := {
-  chanG_tokG :: inG Σ (exclR unitO);
+  chanG_lockG :: lockG Σ;
   chanG_protoG :: protoG Σ val;
 }.
-Definition chanΣ : gFunctors := #[ protoΣ val; GFunctor (exclR unitO) ].
+Definition chanΣ : gFunctors := #[ spin_lockΣ; protoΣ val ].
 Global Instance subG_chanΣ {Σ} : subG chanΣ Σ → chanG Σ.
 Proof. solve_inG. Qed.
+
+Record chan_name := ChanName {
+  chan_lock_name : gname;
+  chan_proto_name : proto_name;
+}.
+Global Instance chan_name_inhabited : Inhabited chan_name :=
+  populate (ChanName inhabitant inhabitant).
+Global Instance chan_name_eq_dec : EqDecision chan_name.
+Proof. solve_decision. Qed.
+Global Instance chan_name_countable : Countable chan_name.
+Proof.
+ refine (inj_countable (λ '(ChanName γl γr), (γl,γr))
+   (λ '(γl, γr), Some (ChanName γl γr)) _); by intros [].
+Qed.
 
 (** * Definition of the pointsto connective *)
 Notation iProto Σ := (iProto Σ val).
 Notation iMsg Σ := (iMsg Σ val).
 
-Definition tok `{!chanG Σ} (γ : gname) : iProp Σ := own γ (Excl ()).
-
-Definition chan_inv `{!heapGS Σ, !chanG Σ} γ γE γt s (l:loc) : iProp Σ :=
-  (l ↦ NONEV ∗ tok γt) ∨
-  (∃ v m, l ↦ SOMEV v ∗
-          iProto_own γ s (<!> m)%proto ∗
-          (∃ p, iMsg_car m v (Next p) ∗ own γE (●E (Next p)))) ∨
-  (∃ p, l ↦ NONEV ∗
-          iProto_own γ s p ∗ own γE (●E (Next p))).
-
 Definition iProto_pointsto_def `{!heapGS Σ, !chanG Σ}
     (c : val) (p : iProto Σ) : iProp Σ :=
-  ∃ γ γE1 γE2 γt1 γt2 s (l1 l2:loc),
-    ⌜ c = PairV #l1 #l2 ⌝ ∗
-    inv (nroot.@"ctx") (iProto_ctx γ) ∗
-    inv (nroot.@"p") (chan_inv γ γE1 γt1 s l1) ∗
-    inv (nroot.@"p") (chan_inv γ γE2 γt2 (side_dual s) l2) ∗
-    own γE1 (●E (Next p)) ∗ own γE1 (◯E (Next p)) ∗
-    iProto_own γ s p.
+  ∃ γ s (l r : loc) (lk : val),
+    ⌜ c = ((#(side_elim s l r), #(side_elim s r l)), lk)%V ⌝ ∗
+    is_lock (chan_lock_name γ) lk (∃ vsl vsr,
+      llist internal_eq l vsl ∗
+      llist internal_eq r vsr ∗
+      steps_lb (length vsl) ∗ steps_lb (length vsr) ∗
+      iProto_ctx (chan_proto_name γ) vsl vsr) ∗
+    iProto_own (chan_proto_name γ) s p.
 Definition iProto_pointsto_aux : seal (@iProto_pointsto_def). by eexists. Qed.
 Definition iProto_pointsto := iProto_pointsto_aux.(unseal).
 Definition iProto_pointsto_eq :
@@ -108,6 +111,25 @@ Arguments iProto_pointsto {_ _ _} _ _%proto.
 Global Instance: Params (@iProto_pointsto) 4 := {}.
 Notation "c ↣ p" := (iProto_pointsto c p)
   (at level 20, format "c  ↣  p").
+
+Global Instance iProto_pointsto_contractive `{!heapGS Σ, !chanG Σ} c :
+  Contractive (iProto_pointsto c).
+Proof. rewrite iProto_pointsto_eq. solve_contractive. Qed.
+
+Definition iProto_choice {Σ} (a : action) (P1 P2 : iProp Σ)
+    (p1 p2 : iProto Σ) : iProto Σ :=
+  (<a @ (b : bool)> MSG #b {{ if b then P1 else P2 }}; if b then p1 else p2)%proto.
+Global Typeclasses Opaque iProto_choice.
+Arguments iProto_choice {_} _ _%I _%I _%proto _%proto.
+Global Instance: Params (@iProto_choice) 2 := {}.
+Infix "<{ P1 }+{ P2 }>" := (iProto_choice Send P1 P2) (at level 85) : proto_scope.
+Infix "<{ P1 }&{ P2 }>" := (iProto_choice Recv P1 P2) (at level 85) : proto_scope.
+Infix "<+{ P2 }>" := (iProto_choice Send True P2) (at level 85) : proto_scope.
+Infix "<&{ P2 }>" := (iProto_choice Recv True P2) (at level 85) : proto_scope.
+Infix "<{ P1 }+>" := (iProto_choice Send P1 True) (at level 85) : proto_scope.
+Infix "<{ P1 }&>" := (iProto_choice Recv P1 True) (at level 85) : proto_scope.
+Infix "<+>" := (iProto_choice Send True True) (at level 85) : proto_scope.
+Infix "<&>" := (iProto_choice Recv True True) (at level 85) : proto_scope.
 
 Section channel.
   Context `{!heapGS Σ, !chanG Σ}.
@@ -119,12 +141,64 @@ Section channel.
   Global Instance iProto_pointsto_proper c : Proper ((≡) ==> (≡)) (iProto_pointsto c).
   Proof. apply (ne_proper _). Qed.
 
-  (* Lemma iProto_pointsto_le c p1 p2 : c ↣ p1 ⊢ ▷ (p1 ⊑ p2) -∗ c ↣ p2. *)
-  (* Proof. *)
-  (*   rewrite iProto_pointsto_eq. iDestruct 1 as (γ s l r lk ->) "[Hlk H]". *)
-  (*   iIntros "Hle'". iExists γ, s, l, r, lk. iSplit; [done|]. iFrame "Hlk". *)
-  (*   by iApply (iProto_own_le with "H"). *)
-  (* Qed. *)
+  Lemma iProto_pointsto_le c p1 p2 : c ↣ p1 ⊢ ▷ (p1 ⊑ p2) -∗ c ↣ p2.
+  Proof.
+    rewrite iProto_pointsto_eq. iDestruct 1 as (γ s l r lk ->) "[Hlk H]".
+    iIntros "Hle'". iExists γ, s, l, r, lk. iSplit; [done|]. iFrame "Hlk".
+    by iApply (iProto_own_le with "H").
+  Qed.
+
+  Global Instance iProto_choice_contractive n a :
+    Proper (dist n ==> dist n ==>
+            dist_later n ==> dist_later n ==> dist n) (@iProto_choice Σ a).
+  Proof. solve_contractive. Qed.
+  Global Instance iProto_choice_ne n a :
+    Proper (dist n ==> dist n ==> dist n ==> dist n ==> dist n) (@iProto_choice Σ a).
+  Proof. solve_proper. Qed.
+  Global Instance iProto_choice_proper a :
+    Proper ((≡) ==> (≡) ==> (≡) ==> (≡) ==> (≡)) (@iProto_choice Σ a).
+  Proof. solve_proper. Qed.
+
+  Lemma iProto_choice_equiv a1 a2 (P11 P12 P21 P22 : iProp Σ)
+        (p11 p12 p21 p22 : iProto Σ) :
+    ⌜a1 = a2⌝ -∗ ((P11 ≡ P12):iProp Σ) -∗ (P21 ≡ P22) -∗
+    ▷ (p11 ≡ p12) -∗ ▷ (p21 ≡ p22) -∗
+    iProto_choice a1 P11 P21 p11 p21 ≡ iProto_choice a2 P12 P22 p12 p22.
+  Proof.
+    iIntros (->) "#HP1 #HP2 #Hp1 #Hp2".
+    rewrite /iProto_choice. iApply iProto_message_equiv; [ eauto | | ].
+    - iIntros "!>" (b) "H". iExists b. iSplit; [ done | ].
+      destruct b;
+        [ iRewrite -"HP1"; iFrame "H Hp1" | iRewrite -"HP2"; iFrame "H Hp2" ].
+    - iIntros "!>" (b) "H". iExists b. iSplit; [ done | ].
+      destruct b;
+        [ iRewrite "HP1"; iFrame "H Hp1" | iRewrite "HP2"; iFrame "H Hp2" ].
+  Qed.
+
+  Lemma iProto_dual_choice a P1 P2 p1 p2 :
+    iProto_dual (iProto_choice a P1 P2 p1 p2)
+    ≡ iProto_choice (action_dual a) P1 P2 (iProto_dual p1) (iProto_dual p2).
+  Proof.
+    rewrite /iProto_choice iProto_dual_message /= iMsg_dual_exist.
+    f_equiv; f_equiv=> -[]; by rewrite iMsg_dual_base.
+  Qed.
+
+  Lemma iProto_app_choice a P1 P2 p1 p2 q :
+    (iProto_choice a P1 P2 p1 p2 <++> q)%proto
+    ≡ (iProto_choice a P1 P2 (p1 <++> q) (p2 <++> q))%proto.
+  Proof.
+    rewrite /iProto_choice iProto_app_message /= iMsg_app_exist.
+    f_equiv; f_equiv=> -[]; by rewrite iMsg_app_base.
+  Qed.
+
+  Lemma iProto_le_choice a P1 P2 p1 p2 p1' p2' :
+    (P1 -∗ P1 ∗ ▷ (p1 ⊑ p1')) ∧ (P2 -∗ P2 ∗ ▷ (p2 ⊑ p2')) -∗
+    iProto_choice a P1 P2 p1 p2 ⊑ iProto_choice a P1 P2 p1' p2'.
+  Proof.
+    iIntros "H". rewrite /iProto_choice. destruct a;
+      iIntros (b) "HP"; iExists b; destruct b;
+      iDestruct ("H" with "HP") as "[$ ?]"; by iModIntro.
+  Qed.
 
   (** ** Specifications of [send] and [recv] *)
   Lemma new_chan_spec p :
@@ -132,36 +206,19 @@ Section channel.
       new_chan #()
     {{{ c1 c2, RET (c1,c2); c1 ↣ p ∗ c2 ↣ iProto_dual p }}}.
   Proof.
-    iIntros (Φ _) "HΦ". wp_lam.
-    wp_alloc l1 as "Hl1".
-    wp_alloc l2 as "Hl2".
+    iIntros (Φ _) "HΦ". wp_lam. iMod (steps_lb_0) as "#Hlb".
+    wp_smart_apply (lnil_spec internal_eq with "[//]"); iIntros (l) "Hl".
+    wp_smart_apply (lnil_spec internal_eq with "[//]"); iIntros (r) "Hr".
     iMod (iProto_init p) as (γp) "(Hctx & Hcl & Hcr)".
-    iMod (own_alloc (●E (Next p) ⋅ ◯E (Next p))) as (γl) "[H●l H◯l]".
-    { by apply excl_auth_valid. }
-    iMod (own_alloc (●E (Next (iProto_dual p)) ⋅ ◯E (Next (iProto_dual p)))) as (γr) "[H●r H◯r]".
-    { by apply excl_auth_valid. }
-    iMod (own_alloc (Excl ())) as (γtl) "Htokl".
-    { done. }
-    iMod (own_alloc (Excl ())) as (γtr) "Htokr".
-    { done. }
-    wp_pures.
-    iMod (inv_alloc _ ⊤ (iProto_ctx γp) with "[Hctx]")
-      as "#IH".
-    { done. }
-    iMod (inv_alloc _ ⊤ (chan_inv γp γl γtl Left l1) with "[Hl1 Htokl]")
-      as "#IHl".
-    { iLeft. iFrame. }
-    iMod (inv_alloc _ ⊤ (chan_inv γp γr γtr Right l2) with "[Hl2 Htokr]")
-      as "#IHr".
-    { iLeft. iFrame. }
-    iModIntro.
-    iApply "HΦ".
-    iSplitL "Hcl H●l H◯l".
-    - rewrite iProto_pointsto_eq.
-      iExists _, _, _, _, _, _, _, _. eauto with iFrame.
-    - rewrite iProto_pointsto_eq.
-      iExists _, _, _, _, _, _, _, _. 
-      iSplit; [done|]. iFrame "#∗". 
+    wp_smart_apply (newlock_spec (∃ vsl vsr,
+      llist internal_eq l vsl ∗ llist internal_eq r vsr ∗
+      steps_lb (length vsl) ∗ steps_lb (length vsr) ∗
+      iProto_ctx γp vsl vsr) with "[Hl Hr Hctx]").
+    { iExists [], []. iFrame "#∗". }
+    iIntros (lk γlk) "#Hlk". wp_pures. iApply "HΦ".
+    set (γ := ChanName γlk γp). iSplitL "Hcl".
+    - rewrite iProto_pointsto_eq. iExists γ, Left, l, r, lk. by iFrame "Hcl #".
+    - rewrite iProto_pointsto_eq. iExists γ, Right, l, r, lk. by iFrame "Hcr #".
   Qed.
 
   Lemma fork_chan_spec p Φ (f : val) :
@@ -176,159 +233,149 @@ Section channel.
     wp_pures. iApply ("HΦ" with "Hc1").
   Qed.
 
-  Lemma own_prot_excl γ (p1 p2 : iProto Σ) :
-    own γ (◯E (Next p1)) -∗ own γ (◯E (Next p2)) -∗ False.
-  Proof. Admitted.
-
   Lemma send_spec c v p :
     {{{ c ↣ <!> MSG v; p }}}
       send c v
     {{{ RET #(); c ↣ p }}}.
   Proof.
     rewrite iProto_pointsto_eq. iIntros (Φ) "Hc HΦ". wp_lam; wp_pures.
-    iDestruct "Hc" as (γ γE1 γE2 γt1 γt2 s l1 l2 ->)
-                        "(#IH & #IHl & #IHr & H● & H◯ & Hown)".
-    wp_pures.
-    wp_bind (Store _ _).
-    iInv "IHl" as "HIp".
-    iDestruct "HIp" as "[HIp|HIp]"; last first.
-    { iDestruct "HIp" as "[HIp|HIp]".
-      - iDestruct "HIp" as (? m) "(>Hl & Hown' & HIp)".
-        wp_store.
-        rewrite /iProto_own.
-        iDestruct "Hown" as (p') "[_ Hown]".
-        iDestruct "Hown'" as (p'') "[_ Hown']".
-        iDestruct (own_prot_excl with "Hown Hown'") as "H". done.
-      - iDestruct "HIp" as (p') "(>Hl & Hown' & HIp)".
-        wp_store.
-        rewrite /iProto_own.
-        iDestruct "Hown" as (p'') "[_ Hown]".
-        iDestruct "Hown'" as (p''') "[_ Hown']".
-        iDestruct (own_prot_excl with "Hown Hown'") as "H". done. }
-    iDestruct "HIp" as "[>Hl Htok]".
-    wp_store.
-    iMod (own_update_2 with "H● H◯") as "[H● H◯]".
-    { apply excl_auth_update. }
-    iModIntro.
-    iSplitL "Hl H● Hown". 
-    { iRight. iLeft. iIntros "!>". iExists _, _. iFrame.
-      iExists _. iFrame. rewrite iMsg_base_eq. simpl. done. }
-    wp_pures.
-    iLöb as "HL".
-    wp_lam.
-    wp_bind (Load _).
-    iInv "IHl" as "HIp".
-    iDestruct "HIp" as "[HIp|HIp]".
-    { iDestruct "HIp" as ">[Hl Htok']".
-      iDestruct (own_valid_2 with "Htok Htok'") as %H. done. }
-    iDestruct "HIp" as "[HIp|HIp]".
-    - iDestruct "HIp" as (? m) "(>Hl & Hown & HIp)".
-      wp_load. iModIntro.
-      iSplitL "Hl Hown HIp".
-      { iRight. iLeft. iExists _, _. iFrame. }
-      wp_pures. iApply ("HL" with "HΦ Htok H◯").
-    - iDestruct "HIp" as (p') "(>Hl & Hown & H●)".
-      wp_load.
-      iModIntro.
-      iSplitL "Hl Htok".
-      { iLeft. iFrame. }
-      iDestruct (own_valid_2 with "H● H◯") as "#Hagree".
-      iDestruct (excl_auth_agreeI with "Hagree") as "Hagree'".
-      wp_pures.
-      iMod (own_update_2 with "H● H◯") as "[H● H◯]".
-      { apply excl_auth_update. }
-      iModIntro.
-      iApply "HΦ".
-      iExists _, _, _, _, _, _, _, _.
-      iSplit; [done|]. iFrame "#∗".
-      iRewrite -"Hagree'". done.
+    iDestruct "Hc" as (γ s l r lk ->) "[#Hlk H]"; wp_pures.
+    wp_smart_apply (acquire_spec with "Hlk"); iIntros "[Hlkd Hinv]".
+    iDestruct "Hinv" as (vsl vsr) "(Hl & Hr & #Hlbl & #Hlbr & Hctx)".
+    destruct s; simpl.
+    - wp_pures. wp_bind (lsnoc _ _).
+      iApply (wp_step_fupdN_lb with "Hlbr [Hctx H]"); [done| |].
+      { iApply fupd_mask_intro; [set_solver|]. simpl.
+        iIntros "Hclose !>!>".
+        iMod (iProto_send_l with "Hctx H []") as "[Hctx H]".
+        { rewrite iMsg_base_eq /=; auto. }
+        iModIntro.
+        iApply step_fupdN_intro; [done|].
+        iIntros "!>". iMod "Hclose".
+        iCombine ("Hctx H") as "H".
+        iExact "H". }
+      iApply (wp_lb_update with "Hlbl").
+      wp_smart_apply (lsnoc_spec with "[$Hl //]"); iIntros "Hl".
+      iIntros "#Hlbl' [Hctx H] !>".
+      wp_smart_apply (release_spec with "[Hl Hr Hctx $Hlk $Hlkd]").
+      { iExists (vsl ++ [v]), vsr.
+        rewrite app_length /=.
+        replace (length vsl + 1) with (S (length vsl)) by lia.
+        iFrame "#∗". }
+      iIntros "_". iApply "HΦ". iExists γ, Left, l, r, lk. eauto 10 with iFrame.
+    - wp_pures. wp_bind (lsnoc _ _).
+      iApply (wp_step_fupdN_lb with "Hlbl [Hctx H]"); [done| |].
+      { iApply fupd_mask_intro; [set_solver|]. simpl.
+        iIntros "Hclose !>!>".
+        iMod (iProto_send_r with "Hctx H []") as "[Hctx H]".
+        { rewrite iMsg_base_eq /=; auto. }
+        iModIntro.
+        iApply step_fupdN_intro; [done|].
+        iIntros "!>". iMod "Hclose".
+        iCombine ("Hctx H") as "H".
+        iExact "H". }
+      iApply (wp_lb_update with "Hlbr").
+      wp_smart_apply (lsnoc_spec with "[$Hr //]"); iIntros "Hr".
+      iIntros "#Hlbr' [Hctx H] !>".
+      wp_smart_apply (release_spec with "[Hl Hr Hctx $Hlk $Hlkd]").
+      { iExists vsl, (vsr ++ [v]).
+        rewrite app_length /=.
+        replace (length vsr + 1) with (S (length vsr)) by lia.
+        iFrame "#∗". }
+      iIntros "_". iApply "HΦ". iExists γ, Right, l, r, lk. eauto 10 with iFrame.
   Qed.
 
-  (* Lemma send_spec_tele {TT} c (tt : TT) *)
-  (*       (v : TT → val) (P : TT → iProp Σ) (p : TT → iProto Σ) : *)
-  (*   {{{ c ↣ (<!.. x > MSG v x {{ P x }}; p x) ∗ P tt }}} *)
-  (*     send c (v tt) *)
-  (*   {{{ RET #(); c ↣ (p tt) }}}. *)
-  (* Proof. *)
-  (*   iIntros (Φ) "[Hc HP] HΦ". *)
-  (*   iDestruct (iProto_pointsto_le _ _ (<!> MSG v tt; p tt)%proto with "Hc [HP]") *)
-  (*     as "Hc". *)
-  (*   { iIntros "!>". *)
-  (*     iApply iProto_le_trans. *)
-  (*     iApply iProto_le_texist_intro_l. *)
-  (*     by iFrame "HP". } *)
-  (*   by iApply (send_spec with "Hc"). *)
-  (* Qed. *)
+  Lemma send_spec_tele {TT} c (tt : TT)
+        (v : TT → val) (P : TT → iProp Σ) (p : TT → iProto Σ) :
+    {{{ c ↣ (<!.. x > MSG v x {{ P x }}; p x) ∗ P tt }}}
+      send c (v tt)
+    {{{ RET #(); c ↣ (p tt) }}}.
+  Proof.
+    iIntros (Φ) "[Hc HP] HΦ".
+    iDestruct (iProto_pointsto_le _ _ (<!> MSG v tt; p tt)%proto with "Hc [HP]")
+      as "Hc".
+    { iIntros "!>".
+      iApply iProto_le_trans.
+      iApply iProto_le_texist_intro_l.
+      by iFrame "HP". }
+    by iApply (send_spec with "Hc").
+  Qed.
+
+  Lemma try_recv_spec {TT} c (v : TT → val) (P : TT → iProp Σ) (p : TT → iProto Σ) :
+    {{{ c ↣ <?.. x> MSG v x {{ P x }}; p x }}}
+      try_recv c
+    {{{ w, RET w; (⌜w = NONEV⌝ ∗ c ↣ <?.. x> MSG v x {{ P x }}; p x) ∨
+                  (∃.. x, ⌜w = SOMEV (v x)⌝ ∗ c ↣ p x ∗ P x) }}}.
+  Proof.
+    rewrite iProto_pointsto_eq. iIntros (Φ) "Hc HΦ". wp_lam; wp_pures.
+    iDestruct "Hc" as (γ s l r lk ->) "[#Hlk H]"; wp_pures.
+    wp_smart_apply (acquire_spec with "Hlk"); iIntros "[Hlkd Hinv]".
+    iDestruct "Hinv" as (vsl vsr) "(Hl & Hr & #Hlbl & #Hlbr & Hctx)". destruct s; simpl.
+    - wp_smart_apply (lisnil_spec with "Hr"); iIntros "Hr".
+      destruct vsr as [|vr vsr]; wp_pures.
+      { wp_smart_apply (release_spec with "[Hl Hr Hctx $Hlk $Hlkd]"); [by eauto with iFrame|].
+        iIntros "_". wp_pures. iModIntro. iApply "HΦ". iLeft. iSplit; [done|].
+        iExists γ, Left, l, r, lk. eauto 10 with iFrame. }
+      wp_smart_apply (lpop_spec with "Hr"); iIntros (v') "[% Hr]"; simplify_eq/=.
+      iMod (iProto_recv_l with "Hctx H") as (q) "(Hctx & H & Hm)". wp_pures.
+      rewrite iMsg_base_eq.
+      iDestruct (iMsg_texist_exist with "Hm") as (x <-) "[Hp HP]".
+      iDestruct (steps_lb_le _ (length vsr) with "Hlbr") as "#Hlbr'"; [lia|].
+      wp_smart_apply (release_spec with "[Hl Hr Hctx $Hlk $Hlkd]"); [by eauto with iFrame|].
+      iIntros "_". wp_pures. iModIntro. iApply "HΦ". iRight. iExists x. iSplit; [done|].
+      iFrame "HP". iExists γ, Left, l, r, lk. iSplit; [done|]. iFrame "Hlk".
+      by iRewrite "Hp".
+    - wp_smart_apply (lisnil_spec with "Hl"); iIntros "Hl".
+      destruct vsl as [|vl vsl]; wp_pures.
+      { wp_smart_apply (release_spec with "[Hl Hr Hctx $Hlk $Hlkd]"); [by eauto with iFrame|].
+        iIntros "_". wp_pures. iModIntro. iApply "HΦ". iLeft. iSplit; [done|].
+        iExists γ, Right, l, r, lk. eauto 10 with iFrame. }
+      wp_smart_apply (lpop_spec with "Hl"); iIntros (v') "[% Hl]"; simplify_eq/=.
+      iMod (iProto_recv_r with "Hctx H") as (q) "(Hctx & H & Hm)". wp_pures.
+      rewrite iMsg_base_eq.
+      iDestruct (iMsg_texist_exist with "Hm") as (x <-) "[Hp HP]".
+      iDestruct (steps_lb_le _ (length vsl) with "Hlbl") as "#Hlbl'"; [lia|].
+      wp_smart_apply (release_spec with "[Hl Hr Hctx $Hlk $Hlkd]"); [by eauto with iFrame|].
+      iIntros "_". wp_pures. iModIntro. iApply "HΦ". iRight. iExists x. iSplit; [done|].
+      iFrame "HP". iExists γ, Right, l, r, lk. iSplit; [done|]. iFrame "Hlk".
+      by iRewrite "Hp".
+  Qed.
 
   Lemma recv_spec {TT} c (v : TT → val) (P : TT → iProp Σ) (p : TT → iProto Σ) :
     {{{ c ↣ <?.. x> MSG v x {{ ▷ P x }}; p x }}}
       recv c
     {{{ x, RET v x; c ↣ p x ∗ P x }}}.
   Proof.
-    iIntros (Φ) "Hc HΦ". iLöb as "HL". wp_lam.
-    rewrite iProto_pointsto_eq.
-    iDestruct "Hc" as (γ E1 γE2 γt1 γt2 s l1 l2 ->)
-                        "(#IH & #IHl & #IHr & H● & H◯ & Hown)".
-    wp_pures.
-    wp_bind (Xchg _ _).
-    iInv "IHr" as "HIp".
-    iDestruct "HIp" as "[HIp|HIp]".
-    { iDestruct "HIp" as ">[Hl Htok]".
-      wp_xchg.
-      iModIntro.
-      iSplitL "Hl Htok".
-      { iLeft. iFrame. }
-      wp_pures. iApply ("HL" with "[H● H◯ Hown] HΦ").
-      iExists _, _, _, _, _, _, _, _. iSplit; [done|]. iFrame "#∗". }
-    iDestruct "HIp" as "[HIp|HIp]"; last first.
-    { iDestruct "HIp" as (p') "[>Hl [Hown' H◯']]".
-      wp_xchg.
-      iModIntro.
-      iSplitL "Hl Hown' H◯'".
-      { iRight. iRight. iExists _. iFrame. }
-      wp_pures. iApply ("HL" with "[H● H◯ Hown] HΦ").
-      iExists _, _, _, _, _, _, _, _. iSplit; [done|]. iFrame "#∗". }
-    iDestruct "HIp" as (w m) "(>Hl & Hown' & HIp)".
-    iDestruct "HIp" as (p') "[Hm Hp']".
-    iInv "IH" as "Hctx".
-    wp_xchg.
-    destruct s.
-    - simpl.
-      iMod (iProto_step_r with "Hctx Hown Hown' Hm") as
-        (p'') "(Hm & Hctx & Hown & Hown')".
-      iModIntro.
-      iSplitL "Hctx"; [done|].
-      iModIntro.
-      iSplitL "Hl Hown' Hp'".
-      { iRight. iRight. iExists _. iFrame. }
-      wp_pure _.
-      rewrite iMsg_base_eq. 
-      iDestruct (iMsg_texist_exist with "Hm") as (x <-) "[Hp HP]".
-      wp_pures. 
-      iMod (own_update_2 with "H● H◯") as "[H● H◯]".
-      { apply excl_auth_update. }
-      iModIntro. iApply "HΦ".
-      iFrame.
-      iExists _, _, _, _, _, _, _, _. iSplit; [done|].
-      iRewrite "Hp". iFrame "#∗". done.
-    - simpl.
-      iMod (iProto_step_l with "Hctx Hown' Hown Hm") as
-        (p'') "(Hm & Hctx & Hown & Hown')".
-      iModIntro.
-      iSplitL "Hctx"; [done|].
-      iModIntro.
-      iSplitL "Hl Hown Hp'".
-      { iRight. iRight. iExists _. iFrame. }
-      wp_pure _.
-      rewrite iMsg_base_eq. 
-      iDestruct (iMsg_texist_exist with "Hm") as (x <-) "[Hp HP]".
-      wp_pures. 
-      iMod (own_update_2 with "H● H◯") as "[H● H◯]".
-      { apply excl_auth_update. }
-      iModIntro. iApply "HΦ".
-      iFrame.
-      iExists _, _, _, _, _, _, _, _. iSplit; [done|].
-      iRewrite "Hp". iFrame "#∗". done.
+    iIntros (Φ) "Hc HΦ". iLöb as "IH". wp_lam.
+    wp_smart_apply (try_recv_spec with "Hc"); iIntros (w) "[[-> H]|H]".
+    { wp_pures. by iApply ("IH" with "[$]"). }
+    iDestruct "H" as (x ->) "[Hc HP]". wp_pures. iApply "HΦ". by iFrame.
   Qed.
 
+  (** ** Specifications for choice *)
+  Lemma select_spec c (b : bool) P1 P2 p1 p2 :
+    {{{ c ↣ (p1 <{P1}+{P2}> p2) ∗ if b then P1 else P2 }}}
+      send c #b
+    {{{ RET #(); c ↣ (if b then p1 else p2) }}}.
+  Proof.
+    rewrite /iProto_choice. iIntros (Φ) "[Hc HP] HΦ".
+    iApply (send_spec with "[Hc HP] HΦ").
+    iApply (iProto_pointsto_le with "Hc").
+    iIntros "!>". iExists b. by iFrame "HP".
+  Qed.
+
+  Lemma branch_spec c P1 P2 p1 p2 :
+    {{{ c ↣ (p1 <{P1}&{P2}> p2) }}}
+      recv c
+    {{{ b, RET #b; c ↣ (if b : bool then p1 else p2) ∗ if b then P1 else P2 }}}.
+  Proof.
+    rewrite /iProto_choice. iIntros (Φ) "Hc HΦ".
+    iApply (recv_spec _ (tele_app _)
+      (tele_app (TT:=[tele _ : bool]) (λ b, if b then P1 else P2))%I
+      (tele_app _) with "[Hc]").
+    { iApply (iProto_pointsto_le with "Hc").
+      iIntros "!> /=" (b) "HP". iExists b. by iSplitL. }
+    rewrite -bi_tforall_forall.
+    iIntros "!>" (x) "[Hc H]". iApply "HΦ". iFrame.
+  Qed.
 End channel.
