multi_actris/channel/proto_model.v
@@ -35,7 +35,7 @@ The defined functions on the type [proto] are:
   all terminations [END] in [p1] with [p2]. *)
 From iris.base_logic Require Import base_logic.
 From iris.proofmode Require Import proofmode.
-From actris.utils Require Import cofe_solver_2.
+From multi_actris.utils Require Import cofe_solver_2.
 Set Default Proof Using "Type".
 
 Module Export action.
